lemma_ends_with_snl1_snl2_implies_snl1_contains_snl2_head - 증명 성공!

src/study/Nemonuri.Study.CSharpSyntaxRewriter2.Modifier/Nemonuri.StratifiedNode.NodeTheory.fst
@@ -8,8 +8,8 @@ let get_level (#t:eqtype) (#lv:pos) (sn:stratified_node t lv) : Tot pos = lv
 
 let is_child 
   (#t:eqtype) 
-  (#child_level:pos) (child:stratified_node t child_level) 
   (#parent_level:pos) (parent:stratified_node t parent_level)
+  (#child_level:pos) (child:stratified_node t child_level) 
   : Tot bool
   = contains parent.children child
 
@@ -20,9 +20,9 @@ let stratified_node_level_is_children_level_plus_one
 
 let lemma_child_node_level_is_lower_than_parent
   (#t:eqtype) 
-  (#child_level:pos) (child:stratified_node t child_level) 
   (#parent_level:pos) (parent:stratified_node t parent_level)
-  : Lemma (requires is_child child parent)
+  (#child_level:pos) (child:stratified_node t child_level) 
+  : Lemma (requires is_child parent child)
           (ensures (child_level < parent_level))
   = let children = parent.children in
     lemma_node_is_element_implies_node_level_is_less_or_equal_than_list_max_level children child
@@ -52,15 +52,86 @@ let stratified_node_is_branch_is_equivalent_to_stratified_node_level_is_greater_
     )
   = ()
 
+let rec sum (l:list nat)
+  : Tot nat
+  = match l with
+  | [] -> 0
+  | hd::tl -> hd + (sum tl)
+
+let is_shorter_or_equal_than_children 
+  (#t:eqtype) (#lv:pos) (parent:stratified_node t lv)
+  (#mlv:nat) (snl:stratified_node_list t mlv)
+  : Tot bool
+  = is_left_shorter_or_equal_than_right snl parent.children
+
+let ends_with_children 
+  (#t:eqtype) (#lv:pos) (parent:stratified_node t lv)
+  (#end_mlv:nat) (end_snl:stratified_node_list t end_mlv{ is_shorter_or_equal_than_children parent end_snl })
+  : Tot bool
+  = ends_with parent.children end_snl
+
+let is_subchildren 
+  (#t:eqtype) (#lv:pos) (parent:stratified_node t lv)
+  (#mlv:nat) (snl:stratified_node_list t mlv)
+  : Tot bool
+  = (is_shorter_or_equal_than_children parent snl) && (ends_with_children parent snl)
+
+let lemma_subchilren_hd_is_child
+  (#t:eqtype) (#lv:pos) (parent:stratified_node t lv) 
+  (#children_mlv:nat)
+  (subchildren:stratified_node_list t children_mlv)
+  : Lemma (requires (not (is_empty subchildren)) && (is_subchildren parent subchildren))
+          (ensures is_child parent (get_hd subchildren))
+  = ()
+
+private let rec select_in_children_core
+  (#t:eqtype) (#lv:pos) (parent:stratified_node t lv) 
+  (#children_mlv:nat)
+  (subchildren:stratified_node_list t children_mlv{ is_subchildren parent subchildren })
+  (#t2:Type) (selector:(#clv:pos -> csn:(stratified_node t clv){ is_child parent csn } -> Tot t2))
+  : Tot (x:(list t2){ L.length x = get_length subchildren }) 
+        (decreases subchildren)
+  = if is_empty subchildren then 
+      []
+    else
+      (
+        //assert ( is_child parent (get_hd subchildren) );
+        let hd = get_hd subchildren in
+        (selector #(get_level hd) hd)::
+        (select_in_children_core parent (get_tl subchildren) selector)
+      )
+
+
+(*
+let rec select_in_children
+  (#t:eqtype) (#lv:pos) (sn:stratified_node t lv) 
+  (#t2:Type) 
+  (selector:(#clv:pos -> csn:(stratified_node t lv){ is_child csn sn } -> Tot t2))
+  : Tot (x:(list t2){ L.length x = get_length sn.children })
+  = let children = sn.children in
+    if is_empty sn.children then []
+    else
+      (selector (get_hd children))::
+      (select )
+*)
+  
+//select sn.children selector
+
+
 (*
 let rec get_count
   (#t:eqtype) (#lv:pos) (sn:stratified_node t lv) 
-  : Tot pos (decreases (get_level sn))
+  : Tot pos (decreases lv)
   = if is_leaf sn then 
       1
     else 
-      L.length (
-        stratified_node_level_is_children_level_plus_one sn;
-        select (SNode?.children sn) get_count
+      sum (
+        select sn.children (
+          fun (#lv2:pos) (sn2:stratified_node t lv2) -> (
+            assert (is_child sn2 sn);
+            lemma_child_node_level_is_lower_than_parent sn2 sn;
+            get_count #t #lv2 sn2
+          )
+        )
       )
 *)
