src/study/Nemonuri.Study.CSharpSyntaxRewriter2.Modifier/Nemonuri.StratifiedNode.ListTheory.Base.fst
@@ -1,0 +1,133 @@
+module Nemonuri.StratifiedNode.ListTheory.Base
+
+module L = FStar.List.Tot.Base
+open Nemonuri.StratifiedNode
+
+let get_max_level (#t:eqtype) (#mlv:nat) (snl:stratified_node_list t mlv) : Tot nat = mlv
+
+let get_hd_level (#t:eqtype) (#lv:pos) (snl:stratified_node_list t lv{SCons? snl})
+  : Tot pos
+  = SCons?.hd_level snl
+
+let get_hd 
+  (#t:eqtype) (#mlv:nat) (snl:stratified_node_list t mlv{SCons? snl}) 
+  : Tot (stratified_node t (get_hd_level snl))
+  = SCons?.hd snl
+
+let get_tl_level (#t:eqtype) (#lv:pos) (snl:stratified_node_list t lv{SCons? snl})
+  : Tot nat
+  = SCons?.tl_level snl
+
+let get_tl
+  (#t:eqtype) (#lv:pos) (snl:stratified_node_list t lv{SCons? snl})
+  : Tot (stratified_node_list t (get_tl_level snl))
+  = SCons?.tl snl
+
+let hd_tl_pair (#t:eqtype) (#lv:pos) (snl:stratified_node_list t lv{SCons? snl}) =
+  stratified_node t (get_hd_level snl) & stratified_node_list t (get_tl_level snl)
+
+let get_hd_tl_pair (#t:eqtype) (#lv:pos) (snl:stratified_node_list t lv{SCons? snl})
+  : Tot (hd_tl_pair snl)
+  = (get_hd snl, get_tl snl)
+
+let try_get_hd_tl (#t:eqtype) (#lv:pos) (snl:stratified_node_list t lv)
+  : Tot (option (hd_tl_pair snl))
+  = if (SCons? snl) then
+      Some (get_hd_tl_pair snl)
+    else
+      None
+
+let is_empty (#t:eqtype) (#mlv:nat) (snl:stratified_node_list t mlv) 
+  : Tot bool
+  = SNil? snl
+
+let rec get_length (#t:eqtype) (#mlv:nat) (snl:stratified_node_list t mlv) 
+  : Tot nat (decreases snl)
+  = if is_empty snl then
+      0
+    else
+      1 + (get_length (get_tl snl))
+
+// 오, 그러고보니 'L.length x = get_length snl' 이게 증명이 되네!
+let rec select 
+  (#t:eqtype) (#mlv:nat) (snl:stratified_node_list t mlv) 
+  (#t2:Type) (selector:(#lv:pos -> stratified_node t lv -> Tot t2))
+  : Tot (x:(list t2){ L.length x = get_length snl }) (decreases snl)
+  = if is_empty snl then []
+    else (selector (get_hd snl))::(select (get_tl snl) selector)
+
+let rec get_node_level
+  (#t:eqtype) (#mlv:nat) (snl:stratified_node_list t mlv)
+  (index:nat{index < (get_length snl)})
+  : Tot pos
+  = if index = 0 then
+      get_hd_level snl
+    else
+      get_node_level (get_tl snl) (index - 1)
+
+let rec get_node
+  (#t:eqtype) (#mlv:nat) (snl:stratified_node_list t mlv)
+  (index:nat{index < (get_length snl)})
+  : Tot (stratified_node t (get_node_level snl index))
+  = if index = 0 then
+      get_hd snl
+    else
+      get_node (get_tl snl) (index - 1)
+
+let is_head 
+  (#t:eqtype) (#mlv:pos) (snl:stratified_node_list t mlv)
+  (#lv:pos) (sn:stratified_node t lv)
+  : Tot bool
+  = ((get_hd_level snl) = lv) && ((get_hd snl) = sn)
+
+let rec contains
+  (#t:eqtype) (#mlv:nat) (snl:stratified_node_list t mlv)
+  (#lv:pos) (sn:stratified_node t lv)
+  : Tot bool
+  = if is_empty snl then
+      false
+    else
+      if is_head snl sn then 
+        true
+      else
+        contains (get_tl snl) sn
+
+let is_left_shorter_or_equal_than_right
+  (#t:eqtype) (#l_mlv:nat) (l_snl:stratified_node_list t l_mlv)
+  (#r_mlv:nat) (r_snl:stratified_node_list t r_mlv)
+  : Tot bool
+  = (get_length l_snl) <= (get_length r_snl)
+
+let is_left_length_is_right_length_minus_one
+  (#t:eqtype) (#l_mlv:nat) (l_snl:stratified_node_list t l_mlv)
+  (#r_mlv:nat) (r_snl:stratified_node_list t r_mlv)
+  : Tot bool
+  = (get_length l_snl) = ((get_length r_snl) - 1)
+
+let is_tail
+  (#t:eqtype) (#mlv:pos) (snl:stratified_node_list t mlv)
+  (#tail_mlv:nat) (tail_snl:stratified_node_list t tail_mlv{ is_left_length_is_right_length_minus_one tail_snl snl })
+  : Tot bool
+  = ((get_tl_level snl) = tail_mlv) && ((get_tl snl) = tail_snl)
+
+let is_equal
+  (#t:eqtype) (#l_mlv:nat) (l_snl:stratified_node_list t l_mlv)
+  (#r_mlv:nat) (r_snl:stratified_node_list t r_mlv)
+  : Tot bool
+  = (l_mlv = r_mlv) && (l_snl = r_snl)
+
+let rec ends_with
+  (#t:eqtype) (#mlv:nat) (snl:stratified_node_list t mlv)
+  (#end_mlv:nat) (end_snl:stratified_node_list t end_mlv{ is_left_shorter_or_equal_than_right end_snl snl })
+  : Tot bool (decreases snl)
+  = if (is_empty end_snl) then true
+    else if (is_equal snl end_snl) then true
+    (* else
+    if (is_left_length_is_right_length_minus_one end_snl snl) then 
+      is_tail snl end_snl *)
+    else
+      let next_snl = get_tl snl in
+      if is_left_shorter_or_equal_than_right end_snl next_snl then
+        ends_with next_snl end_snl
+      else
+        false
