src/study/Nemonuri.Study.CSharpSyntaxRewriter2.Modifier/Nemonuri.StratifiedNode.ListTheory.Properties.fst
@@ -1,0 +1,107 @@
+module Nemonuri.StratifiedNode.ListTheory.Properties
+
+module L = FStar.List.Tot.Base
+open Nemonuri.StratifiedNode.ListTheory.Base
+open Nemonuri.StratifiedNode
+
+let lemma_stratified_node_list_which_max_level_is_zero_has_no_elements
+  (#t:eqtype) (#mlv:nat) (snl:stratified_node_list t mlv)
+  : Lemma (requires get_max_level snl = 0)
+          (ensures SNil? snl)
+  = ()
+
+let rec lemma_stratified_node_list_which_max_level_greater_than_zero_has_a_element_which_level_is_max_level
+  (#t:eqtype) (#mlv:nat) (snl:stratified_node_list t mlv)
+  : Lemma (requires get_max_level snl > 0)
+          (ensures 
+            (SCons? snl) /\
+            (
+              ((get_hd_level snl) = (get_max_level snl)) \/
+              ((get_tl_level snl) = (get_max_level snl))
+            )
+          )
+          (decreases snl)
+  = if SNil? (get_tl snl) then 
+      ()
+    else
+      lemma_stratified_node_list_which_max_level_greater_than_zero_has_a_element_which_level_is_max_level (get_tl snl)
+
+let lemma_head_level_is_less_or_equal_then_list_max_level
+  (#t:eqtype) (#mlv:pos) (snl:stratified_node_list t mlv)
+  (#lv:pos) (sn:stratified_node t lv)
+  : Lemma (requires is_head snl sn)
+          (ensures lv <= mlv)
+  = ()
+
+let lemma_node_is_head_implies_node_is_element
+  (#t:eqtype) (#mlv:pos) (snl:stratified_node_list t mlv)
+  (#lv:pos) (sn:stratified_node t lv)
+  : Lemma (ensures ((is_head snl sn) ==> (contains snl sn)))
+  = ()
+
+let rec lemma_node_is_element_implies_node_level_is_less_or_equal_than_list_max_level
+  (#t:eqtype) (#mlv:pos) (snl:stratified_node_list t mlv)
+  (#lv:pos) (sn:stratified_node t lv)
+  : Lemma (ensures (contains snl sn) ==> (lv <= mlv)) (decreases snl)
+  = if (is_head snl sn) then
+      (
+        (* 음...둘 중 하나만 있어도 되네? *)
+        lemma_head_level_is_less_or_equal_then_list_max_level snl sn;
+        lemma_node_is_head_implies_node_is_element snl sn
+      )
+    else
+      let tl = get_tl snl in
+      let tl_level = get_max_level tl in
+      if tl_level = 0 then ()
+      else lemma_node_is_element_implies_node_level_is_less_or_equal_than_list_max_level tl sn
+
+let lemma_element_level_is_less_or_equal_than_list_max_level
+  (#t:eqtype) (#mlv:pos) (snl:stratified_node_list t mlv)
+  (#lv:pos) (sn:stratified_node t lv)
+  : Lemma (requires contains snl sn)
+          (ensures lv <= mlv)
+  = lemma_node_is_element_implies_node_level_is_less_or_equal_than_list_max_level snl sn
+
+let lemma_two_list_are_equal_is_equivalent_to_two_heads_are_equal
+  (#t:eqtype) (#l_mlv:nat) (l_snl:stratified_node_list t l_mlv{SCons? l_snl})
+  (#r_mlv:nat) (r_snl:stratified_node_list t r_mlv{SCons? r_snl})
+  : Lemma (requires is_equal l_snl r_snl)
+          (ensures (get_hd l_snl) = (get_hd r_snl))
+  = ()
+
+let rec lemma_ends_with_snl1_snl2_implies_snl1_contains_snl2_head
+  (#t:eqtype) (#mlv1:nat) (snl1:stratified_node_list t mlv1{SCons? snl1})
+  (#mlv2:nat) (snl2:stratified_node_list t mlv2{SCons? snl2})
+  : Lemma (requires (is_left_shorter_or_equal_than_right snl2 snl1) &&
+                    (ends_with snl1 snl2) )
+          (ensures contains snl1 (get_hd snl2))
+          (decreases snl1)
+  = if (is_equal snl1 snl2) then
+      (
+        lemma_two_list_are_equal_is_equivalent_to_two_heads_are_equal snl1 snl2
+      )
+    else
+      lemma_ends_with_snl1_snl2_implies_snl1_contains_snl2_head (get_tl snl1) snl2
+
+(*
+let rec lemma_ends_with_snl1_snl2_implies_snl1_contains_snl2_head
+  (#t:eqtype) (#mlv1:nat) (snl1:stratified_node_list t mlv1)
+  (#mlv2:nat) (snl2:stratified_node_list t mlv2)
+  : Lemma (ensures 
+            (
+              (not (is_empty snl2)) &&
+              (is_left_shorter_or_equal_than_right snl2 snl1) && 
+              (ends_with snl1 snl2)
+            ) ==>
+            (contains snl1 (get_hd snl2))
+          )
+          (decreases snl2)
+  = if (is_empty snl2) then ()
+    else if not (
+      (not (is_empty snl2)) &&
+      (is_left_shorter_or_equal_than_right snl2 snl1) && 
+      (ends_with snl1 snl2)
+    ) 
+    then (lemma_ends_with_snl1_snl2_implies_snl1_contains_snl2_head snl1 (get_tl snl2))
+    else
+*)
